Added cv Store computation and theorem

examples/compute/src/shared/cv/bir_cv_memScript.sml
@@ -73,6 +73,45 @@ Definition bir_cv_compute_load_def:
 End
 
 
+(* ***************************************** *)
+(* ***************** STORE ***************** *)
+(* ***************************************** *)
+
+
+(* Add all the bitstrings in the mmap at address a *)
+Definition bir_cv_update_mmap_def:
+  (bir_cv_update_mmap aty mmap_alist a [] = mmap_alist) /\
+  (bir_cv_update_mmap aty mmap_alist a (v::vs) =
+    bir_cv_update_mmap aty (((bir_mem_addr aty a), v2n v)::mmap_alist) (SUC a) vs)
+End
+
+
+(* Compute an already unpacked store expression *)
+Definition bir_cv_compute_store_in_mem_def:
+  bir_cv_compute_store_in_mem
+  (vty : bir_immtype_t) (aty : bir_immtype_t) (result : bir_imm_t) (mmap_alist : (num # num) list) (en: bir_endian_t) (addr:num) =
+
+   let rty = type_of_bir_imm result in
+   case (bir_number_of_mem_splits vty rty aty) of
+    | NONE => NONE
+    | SOME (n:num) => (
+        let vs = bitstring_split (size_of_bir_immtype vty) (b2v result) in
+        let vs' = (case en of BEnd_LittleEndian => SOME (REVERSE vs)
+                          |  BEnd_BigEndian => SOME vs
+                          |  BEnd_NoEndian => if (n = 1) then SOME vs else NONE) in
+
+        case vs' of NONE => NONE
+                 |  SOME vs'' => SOME (BCVVal_Mem aty vty (bir_cv_update_mmap aty mmap_alist addr vs''))
+   )
+End
+
+
+Definition bir_cv_compute_store_def:
+  (bir_cv_compute_store (SOME (BCVVal_Mem aty vty mmap_alist)) (SOME (BCVVal_Imm addr)) en (SOME (BCVVal_Imm result)) = 
+    bir_cv_compute_store_in_mem vty aty result mmap_alist en (b2n addr)) /\
+  (bir_cv_compute_store _ _ _ _ = NONE)
+End
+
 (* ****************************************** *)
 (* **************** THEOREMS **************** *)
 (* ****************************************** *)
@@ -131,5 +170,37 @@ Proof
     rw [bir_compute_load_from_mem_alist_to_fmap] >>
     rw [val_from_cv_val_option_from_imm_option]
 QED
+
+(* ***************************************** *)
+(* ***************** STORE ***************** *)
+(* ***************************************** *)
+
+Theorem bir_cv_update_mmap_eq_update_mmap:
+  !aty mmap_alist a l.
+    alist_to_fmap (bir_cv_update_mmap aty mmap_alist a l) =
+      bir_update_mmap aty (alist_to_fmap mmap_alist) a l
+Proof
+  Induct_on `l` >>
+  rw [bir_cv_update_mmap_def, bir_update_mmap_def]
+QED
+
+(* compute and cv_compute are similar *)
+Theorem bir_cv_compute_store_eq_compute_store:
+  !v_mem v_addr en result.
+    from_cv_val_option (bir_cv_compute_store v_mem v_addr en result) =
+    (bir_compute_store (from_cv_val_option v_mem) (from_cv_val_option v_addr) en (from_cv_val_option result))
+Proof
+  Cases_on `v_mem` >> Cases_on `v_addr` >> Cases_on `en` >> Cases_on `result` >>
+    TRY (Cases_on `x`) >> TRY (Cases_on `x'`) >> TRY (Cases_on `x''`) >>
+    rw [from_cv_val_option_def, from_cv_val_def] >>
+    rw [bir_cv_compute_store_def, bir_cv_compute_store_in_mem_def] >>
+    rw [bir_compute_store_def, bir_compute_store_in_mem_def] >>
+    rw [from_cv_val_option_def, from_cv_val_def] >>
+
+    Cases_on `bir_number_of_mem_splits b0 (type_of_bir_imm b'') b` >>
+      rw [from_cv_val_option_def, from_cv_val_def] >>
+      rw [bir_cv_update_mmap_eq_update_mmap]
+QED
+
 
 val _ = export_theory () ;
